Make operational.v work

theories/dotsyn.v
@@ -36,333 +36,405 @@ Inductive tm  : Type :=
   | TSelA : path -> label -> ty -> ty -> ty
   | TNat :  ty.
 
- Instance Ids_tm : Ids tm := λ _, tv (vnat 0).
- Instance Ids_dm : Ids dm := λ _, dvl (vnat 0).
- Instance Ids_pth : Ids path := λ _, pv (vnat 0).
- Instance Ids_ty : Ids ty := λ _, TNat.
+Definition vls := list vl.
+Definition dms := list dm.
 
- Instance Ids_vl : Ids vl.
- Proof. by constructor. Defined.
+Instance Ids_tm : Ids tm := λ _, tv (vnat 0).
+Instance Ids_dm : Ids dm := λ _, dvl (vnat 0).
+Instance Ids_pth : Ids path := λ _, pv (vnat 0).
+Instance Ids_ty : Ids ty := λ _, TNat.
+Instance Ids_vls : Ids vls := λ _, [].
+Instance Ids_dms : Ids dms := λ _, [].
 
- Fixpoint tm_rename (sb : var → var) (e : tm) : tm :=
-   let a := tm_rename : Rename tm in
-   let b := vl_rename : Rename vl in
-   match e with
-   | tv v => tv (rename sb v)
-   | tapp t1 t2 => tapp (rename sb t1) (rename sb t2)
-   | tproj t l => (tproj (rename sb t) l)
-   | tskip t => tskip (rename sb t)
-   end
- with
- vl_rename (sb : var → var) (v : vl) : vl :=
-   let a := tm_rename : Rename tm in
-   let b := vl_rename : Rename vl in
-   let c := dm_rename : Rename dm in
-   match v with
-   | var_vl x => var_vl (sb x)
-   | vnat n => vnat n
-   | vabs t => vabs (rename (upren sb) t)
-   | vobj d => vobj (map (rename (upren sb)) d)
-   end
- with
- dm_rename (sb : var → var) (d : dm) : dm :=
-   let a := vl_rename : Rename vl in
-   let b := ty_rename : Rename ty in
-   match d with
-   | dtysyn ty => dtysyn (rename sb ty)
-   | dtysem lv γ => dtysem (map (rename sb) lv) γ
-   | dvl v => dvl (rename sb v)
-   end
- with
- ty_rename (sb : var → var) (T : ty) : ty :=
-   let a := ty_rename : Rename ty in
-   let b := pth_rename : Rename path in
-   match T with
-   | TTop => TTop
-   | TBot => TBot
-   | TAnd T1 T2 => TAnd (rename sb T1) (rename sb T2)
-   | TOr T1 T2 => TOr (rename sb T1) (rename sb T2)
-   | TLater T => TLater (rename sb T)
-   | TAll T1 T2 => TAll (rename sb T1) (rename (upren sb) T2)
-   | TMu T => TMu (rename (upren sb) T)
-   | TVMem l T => TVMem l (rename sb T)
-   | TTMem l T1 T2 => TTMem l (rename sb T1) (rename sb T2)
-   | TSel pth l => TSel (rename sb pth) l
-   | TSelA pth l T1 T2 => TSelA (rename sb pth) l (rename sb T1) (rename sb T2)
-   | TNat => TNat
-   end
- with
- pth_rename (sb : var → var) (pth : path) : path :=
-   let a := vl_rename : Rename vl in
-   let b := pth_rename : Rename path in
-   match pth with
-   | pv v => pv (rename sb v)
-   | pself pth l => pself (rename sb pth) l
-   end.
+Instance Ids_vl : Ids vl.
+Proof. by constructor. Defined.
 
- Instance Rename_tm : Rename tm := tm_rename.
- Instance Rename_vl : Rename vl := vl_rename.
- Instance Rename_ty : Rename ty := ty_rename.
- Instance Rename_dm : Rename dm := dm_rename.
- Instance Rename_pth : Rename path := pth_rename.
+Definition vls_rename `{Rename vl} (sb : var → var) (vs : vls) : vls :=
+  map (rename sb) vs.
 
- Fixpoint tm_hsubst (sb : var → vl) (e : tm) : tm :=
-   let a := tm_hsubst : HSubst vl tm in
-   let b := vl_subst : Subst vl in
-   match e with
-   | tv v => tv (subst sb v)
-   | tapp t1 t2 => tapp (hsubst sb t1) (hsubst sb t2)
-   | tproj t l => (tproj (hsubst sb t) l)
-   | tskip t => tskip (hsubst sb t)
-   end
- with
- vl_subst (sb : var → vl) (v : vl) : vl :=
-   let a := tm_hsubst : HSubst vl tm in
-   let b := dm_hsubst : HSubst vl dm in
-   match v with
-   | var_vl x => sb x
-   | vnat n => vnat n
-   | vabs t => vabs (hsubst (up sb) t)
-   | vobj d => vobj (map (hsubst (up sb)) d)
-   end
- with
- dm_hsubst (sb : var → vl) (d : dm) : dm :=
-   let a := vl_subst : Subst vl in
-   let b := ty_hsubst : HSubst vl ty in
-   match d with
-   | dtysyn ty => dtysyn (hsubst sb ty)
-   | dtysem lv γ => dtysem (map (subst sb) lv) γ
-   | dvl v => dvl (subst sb v)
-   end
- with
- ty_hsubst (sb : var → vl) (T : ty) : ty :=
+Definition dms_rename `{Rename dm} (sb : var → var) (ds : dms) : dms :=
+  map (rename sb) ds.
+
+Fixpoint tm_rename (sb : var → var) (e : tm) {struct e} : tm :=
+  let a := tm_rename : Rename tm in
+  let b := vl_rename : Rename vl in
+  match e with
+  | tv v => tv (rename sb v)
+  | tapp t1 t2 => tapp (rename sb t1) (rename sb t2)
+  | tproj t l => (tproj (rename sb t) l)
+  | tskip t => tskip (rename sb t)
+  end
+with
+vl_rename (sb : var → var) (v : vl) {struct v} : vl :=
+  let a := tm_rename : Rename tm in
+  let b := vl_rename : Rename vl in
+  let c := dm_rename : Rename dm in
+  let d := dms_rename : Rename dms in
+  match v with
+  | var_vl x => var_vl (sb x)
+  | vnat n => vnat n
+  | vabs t => vabs (rename (upren sb) t)
+  | vobj d => vobj (rename (upren sb) d)
+  end
+with
+dm_rename (sb : var → var) (d : dm) {struct d} : dm :=
+  let a := vl_rename : Rename vl in
+  let b := ty_rename : Rename ty in
+  let c := vls_rename : Rename vls in
+  match d with
+  | dtysyn ty => dtysyn (rename sb ty)
+  | dtysem lv γ => dtysem (rename sb lv) γ
+  | dvl v => dvl (rename sb v)
+  end
+with
+ty_rename (sb : var → var) (T : ty) {struct T}: ty :=
+  let a := ty_rename : Rename ty in
+  let b := path_rename : Rename path in
+  match T with
+  | TTop => TTop
+  | TBot => TBot
+  | TAnd T1 T2 => TAnd (rename sb T1) (rename sb T2)
+  | TOr T1 T2 => TOr (rename sb T1) (rename sb T2)
+  | TLater T => TLater (rename sb T)
+  | TAll T1 T2 => TAll (rename sb T1) (rename (upren sb) T2)
+  | TMu T => TMu (rename (upren sb) T)
+  | TVMem l T => TVMem l (rename sb T)
+  | TTMem l T1 T2 => TTMem l (rename sb T1) (rename sb T2)
+  | TSel pth l => TSel (rename sb pth) l
+  | TSelA pth l T1 T2 => TSelA (rename sb pth) l (rename sb T1) (rename sb T2)
+  | TNat => TNat
+  end
+with
+path_rename (sb : var → var) (pth : path) {struct pth} : path :=
+  let a := vl_rename : Rename vl in
+  let b := path_rename : Rename path in
+  match pth with
+  | pv v => pv (rename sb v)
+  | pself pth l => pself (rename sb pth) l
+  end.
+
+Instance Rename_tm : Rename tm := tm_rename.
+Instance Rename_vl : Rename vl := vl_rename.
+Instance Rename_ty : Rename ty := ty_rename.
+Instance Rename_dm : Rename dm := dm_rename.
+Instance Rename_pth : Rename path := path_rename.
+Instance Rename_vls : Rename vls := vls_rename.
+Instance Rename_dms : Rename dms := dms_rename.
+
+Definition vls_hsubst `{Subst vl} (sb : var → vl) (vs : vls) : vls :=
+  map (subst sb) vs.
+
+Definition dms_hsubst `{HSubst vl dm} (sb : var → vl) (ds : dms) : dms :=
+  map (hsubst sb) ds.
+
+Fixpoint tm_hsubst (sb : var → vl) (e : tm) : tm :=
+  let a := tm_hsubst : HSubst vl tm in
+  let b := vl_subst : Subst vl in
+  match e with
+  | tv v => tv (subst sb v)
+  | tapp t1 t2 => tapp (hsubst sb t1) (hsubst sb t2)
+  | tproj t l => (tproj (hsubst sb t) l)
+  | tskip t => tskip (hsubst sb t)
+  end
+with
+vl_subst (sb : var → vl) (v : vl) : vl :=
+  let a := tm_hsubst : HSubst vl tm in
+  let b := dm_hsubst : HSubst vl dm in
+  let d := dms_hsubst : HSubst vl dms in
+  match v with
+  | var_vl x => sb x
+  | vnat n => vnat n
+  | vabs t => vabs (hsubst (up sb) t)
+  | vobj d => vobj (hsubst (up sb) d)
+  end
+with
+dm_hsubst (sb : var → vl) (d : dm) : dm :=
+  let a := vl_subst : Subst vl in
+  let b := ty_hsubst : HSubst vl ty in
+  let c := vls_hsubst : HSubst vl vls in
+  match d with
+  | dtysyn ty => dtysyn (hsubst sb ty)
+  | dtysem lv γ => dtysem (hsubst sb lv) γ
+  | dvl v => dvl (subst sb v)
+  end
+with
+ty_hsubst (sb : var → vl) (T : ty) : ty :=
   let a := ty_hsubst : HSubst vl ty in
-  let b := pth_hsubst : HSubst vl path in
-   match T with
-   | TTop => TTop
-   | TBot => TBot
-   | TAnd T1 T2 => TAnd (hsubst sb T1) (hsubst sb T2)
-   | TOr T1 T2 => TOr (hsubst sb T1) (hsubst sb T2)
-   | TLater T => TLater (hsubst sb T)
-   | TAll T1 T2 => TAll (hsubst sb T1) (hsubst (up sb) T2)
-   | TMu T => TMu (hsubst (up sb) T)
-   | TVMem l T => TVMem l (hsubst sb T)
-   | TTMem l T1 T2 => TTMem l (hsubst sb T1) (hsubst sb T2)
-   | TSel pth l => TSel (hsubst sb pth) l
-   | TSelA pth l T1 T2 => TSelA (hsubst sb pth) l (hsubst sb T1) (hsubst sb T2)
-   | TNat => TNat
-   end
- with
- pth_hsubst (sb : var → vl) (pth : path) : path :=
-   let b := vl_subst : Subst vl in
- let b := pth_hsubst : HSubst vl path in
-   match pth with
-   | pv v => pv (subst sb v)
-   | pself pth l => pself (hsubst sb pth) l
-   end.
+  let b := path_hsubst : HSubst vl path in
+  match T with
+  | TTop => TTop
+  | TBot => TBot
+  | TAnd T1 T2 => TAnd (hsubst sb T1) (hsubst sb T2)
+  | TOr T1 T2 => TOr (hsubst sb T1) (hsubst sb T2)
+  | TLater T => TLater (hsubst sb T)
+  | TAll T1 T2 => TAll (hsubst sb T1) (hsubst (up sb) T2)
+  | TMu T => TMu (hsubst (up sb) T)
+  | TVMem l T => TVMem l (hsubst sb T)
+  | TTMem l T1 T2 => TTMem l (hsubst sb T1) (hsubst sb T2)
+  | TSel pth l => TSel (hsubst sb pth) l
+  | TSelA pth l T1 T2 => TSelA (hsubst sb pth) l (hsubst sb T1) (hsubst sb T2)
+  | TNat => TNat
+  end
+with
+path_hsubst (sb : var → vl) (pth : path) : path :=
+  let b := vl_subst : Subst vl in
+  let b := path_hsubst : HSubst vl path in
+  match pth with
+  | pv v => pv (subst sb v)
+  | pself pth l => pself (hsubst sb pth) l
+  end.
 
- Instance HSubst_tm : HSubst vl tm := tm_hsubst.
- Instance Subst_vl : Subst vl := vl_subst.
- Instance HSubst_ty : HSubst vl ty := ty_hsubst.
- Instance HSubst_dm : HSubst vl dm := dm_hsubst.
- Instance HSubst_pth : HSubst vl path := pth_hsubst.
+Instance HSubst_tm : HSubst vl tm := tm_hsubst.
+Instance Subst_vl : Subst vl := vl_subst.
+Instance HSubst_ty : HSubst vl ty := ty_hsubst.
+Instance HSubst_dm : HSubst vl dm := dm_hsubst.
+Instance HSubst_pth : HSubst vl path := path_hsubst.
+Instance HSubst_vls : HSubst vl vls := vls_hsubst.
+Instance HSubst_dms : HSubst vl dms := dms_hsubst.
 
 Lemma vl_eq_dec (v1 v2 : vl) : Decision (v1 = v2)
- with
- tm_eq_dec (t1 t2 : tm) : Decision (t1 = t2)
- with
- dm_eq_dec (d1 d2 : dm) : Decision (d1 = d2)
- with
- ty_eq_dec (ty1 ty2 : ty) : Decision (ty1 = ty2)
- with
- pth_eq_dec (pth1 pth2 : path) : Decision (pth1 = pth2).
- Proof.
-   - rewrite /Decision; decide equality;
-       try (apply tm_eq_dec || apply nat_eq_dec || apply @list_eq_dec); auto.
-   - rewrite /Decision; decide equality; try (apply vl_eq_dec || apply nat_eq_dec).
-   - rewrite /Decision; decide equality;
-       try (apply ty_eq_dec || apply vl_eq_dec || apply @list_eq_dec ||
-            apply positive_eq_dec); auto.
-   - rewrite /Decision; decide equality;
-       try (apply pth_eq_dec || apply nat_eq_dec); auto.
-   -  rewrite /Decision; decide equality;
+with
+tm_eq_dec (t1 t2 : tm) : Decision (t1 = t2)
+with
+dm_eq_dec (d1 d2 : dm) : Decision (d1 = d2)
+with
+ty_eq_dec (ty1 ty2 : ty) : Decision (ty1 = ty2)
+with
+path_eq_dec (pth1 pth2 : path) : Decision (pth1 = pth2).
+Proof.
+  - rewrite /Decision; decide equality;
+      try (apply tm_eq_dec || apply nat_eq_dec || apply @list_eq_dec); auto.
+  - rewrite /Decision; decide equality; try (apply vl_eq_dec || apply nat_eq_dec).
+  - rewrite /Decision; decide equality;
+      try (apply ty_eq_dec || apply vl_eq_dec || apply @list_eq_dec ||
+           apply positive_eq_dec); auto.
+  - rewrite /Decision; decide equality;
+      try (apply path_eq_dec || apply nat_eq_dec); auto.
+  -  rewrite /Decision; decide equality;
        try (apply vl_eq_dec || apply nat_eq_dec); auto.
- Qed.
+Qed.
 
- Lemma vl_rename_Lemma (ξ : var → var) (v : vl) : rename ξ v = v.[ren ξ]
- with
- tm_rename_Lemma (ξ : var → var) (t : tm) : rename ξ t = t.|[ren ξ]
- with
- dm_rename_Lemma (ξ : var → var) (d : dm) : rename ξ d = d.|[ren ξ]
- with
- ty_rename_Lemma (ξ : var → var) (T : ty) : rename ξ T = T.|[ren ξ]
- with
- pth_rename_Lemma (ξ : var → var) (pth : path) :
-   rename ξ pth = pth.|[ren ξ].
- Proof.
-   - destruct v; simpl; auto.
-     + by rewrite tm_rename_Lemma up_upren_internal.
-     + f_equal; induction l; simpl; first trivial.
-       by rewrite IHl dm_rename_Lemma up_upren_internal.
-   - destruct t; simpl; auto;
-       try (by rewrite ?vl_rename_Lemma ?tm_rename_Lemma).
-   - destruct d; simpl.
-     + by rewrite ty_rename_Lemma.
-     + f_equal. induction l; simpl; first trivial.
-       by rewrite IHl vl_rename_Lemma.
-     + by rewrite vl_rename_Lemma.
-   - destruct T; simpl; auto;
-       by rewrite ?ty_rename_Lemma ?pth_rename_Lemma ?up_upren_internal.
-   - induction pth; simpl; auto; by rewrite ?vl_rename_Lemma ?pth_rename_Lemma.
- Qed.
+Global Instance vl_eq_dec' : EqDecision vl.
+Proof. by intros ? ?; apply vl_eq_dec. Qed.
+Global Instance tm_eq_dec' : EqDecision tm.
+Proof. by intros ? ?; apply tm_eq_dec. Qed.
+Global Instance dm_eq_dec' : EqDecision dm.
+Proof. by intros ? ?; apply dm_eq_dec. Qed.
+Global Instance ty_eq_dec' : EqDecision ty.
+Proof. by intros ? ?; apply ty_eq_dec. Qed.
+Global Instance path_eq_dec' : EqDecision path.
+Proof. by intros ? ?; apply path_eq_dec. Qed.
+Global Instance vls_eq_dec' : EqDecision vls.
+Proof. by intros ? ?; apply list_eq_dec. Qed.
+Global Instance dms_eq_dec' : EqDecision dms.
+Proof. by intros ? ?; apply list_eq_dec. Qed.
 
- Lemma vl_ids_Lemma (v : vl) : v.[ids] = v
- with
- tm_ids_Lemma (t : tm) : t.|[ids] = t
- with
- dm_ids_Lemma (d : dm) : d.|[ids] = d
- with
- ty_ids_Lemma (T : ty) : T.|[ids] = T
- with
- pth_ids_Lemma (pth : path) : pth.|[ids] = pth.
- Proof.
-   - destruct v; simpl; auto.
-     + by rewrite up_id_internal // tm_ids_Lemma.
-     + f_equal; induction l; simpl; first trivial.
-       by rewrite IHl up_id_internal // dm_ids_Lemma.
-   - destruct t; simpl; auto; by rewrite ?vl_ids_Lemma ?tm_ids_Lemma.
-   - destruct d; simpl.
-     + by rewrite ty_ids_Lemma.
-     + f_equal. induction l; simpl; first trivial.
-       by rewrite IHl vl_ids_Lemma.
-     + by rewrite vl_ids_Lemma.
-   - destruct T; simpl; auto;
-       by rewrite ?ty_ids_Lemma ?up_id_internal // ?ty_ids_Lemma ?pth_ids_Lemma.
-   - induction pth; simpl; auto; by rewrite ?vl_ids_Lemma ?pth_ids_Lemma.
- Qed.
+Lemma vl_rename_Lemma (ξ : var → var) (v : vl) : rename ξ v = v.[ren ξ]
+with
+tm_rename_Lemma (ξ : var → var) (t : tm) : rename ξ t = t.|[ren ξ]
+with
+dm_rename_Lemma (ξ : var → var) (d : dm) : rename ξ d = d.|[ren ξ]
+with
+ty_rename_Lemma (ξ : var → var) (T : ty) : rename ξ T = T.|[ren ξ]
+with
+path_rename_Lemma (ξ : var → var) (pth : path) :
+  rename ξ pth = pth.|[ren ξ].
+Proof.
+  - destruct v; simpl; auto.
+    + by rewrite tm_rename_Lemma up_upren_internal.
+    + rewrite /rename /dms_rename.
+      f_equal; induction l; simpl; first trivial.
+        by rewrite IHl dm_rename_Lemma up_upren_internal.
+  - destruct t; simpl; auto;
+      try (by rewrite ?vl_rename_Lemma ?tm_rename_Lemma).
+  - destruct d; simpl.
+    + by rewrite ty_rename_Lemma.
+    + rewrite /rename /vls_rename.
+      f_equal. induction l; simpl; first trivial.
+        by rewrite IHl vl_rename_Lemma.
+    + by rewrite vl_rename_Lemma.
+  - destruct T; simpl; auto;
+      by rewrite ?ty_rename_Lemma ?path_rename_Lemma ?up_upren_internal.
+  - induction pth; simpl; auto; by rewrite ?vl_rename_Lemma ?path_rename_Lemma.
+Qed.
 
- Lemma vl_comp_rename_Lemma (ξ : var → var) (σ : var → vl) (v : vl) :
-   (rename ξ v).[σ] = v.[ξ >>> σ]
- with
- tm_comp_rename_Lemma (ξ : var → var) (σ : var → vl) (t : tm) :
-   (rename ξ t).|[σ] = t.|[ξ >>> σ]
- with
- dm_comp_rename_Lemma (ξ : var → var) (σ : var → vl) (d : dm) :
-   (rename ξ d).|[σ] = d.|[ξ >>> σ]
- with
- ty_comp_rename_Lemma (ξ : var → var) (σ : var → vl) (T : ty) :
-   (rename ξ T).|[σ] = T.|[ξ >>> σ]
- with
- pth_comp_rename_Lemma (ξ : var → var) (σ : var → vl) (pth : path) :
-   (rename ξ pth).|[σ] = pth.|[ξ >>> σ].
- Proof.
-   - destruct v; simpl; auto.
-     + by rewrite tm_comp_rename_Lemma up_comp_ren_subst.
-     + f_equal; induction l; simpl; first trivial.
-       by rewrite IHl dm_comp_rename_Lemma up_comp_ren_subst.
-   - destruct t; simpl; auto;
-       by rewrite ?vl_comp_rename_Lemma ?tm_comp_rename_Lemma.
-   - destruct d; simpl.
-     + by rewrite ty_comp_rename_Lemma.
-     + f_equal. induction l; simpl; first trivial.
-       by rewrite IHl vl_comp_rename_Lemma.
-     + by rewrite vl_comp_rename_Lemma.
-   - destruct T; simpl; auto;
-       rewrite ?ty_comp_rename_Lemma ?pth_comp_rename_Lemma;
-         by try rewrite up_comp_ren_subst.
-   - induction pth; simpl; auto;
-       by rewrite ?vl_comp_rename_Lemma ?pth_comp_rename_Lemma.
- Qed.
+Lemma vl_ids_Lemma (v : vl) : v.[ids] = v
+with
+tm_ids_Lemma (t : tm) : t.|[ids] = t
+with
+dm_ids_Lemma (d : dm) : d.|[ids] = d
+with
+ty_ids_Lemma (T : ty) : T.|[ids] = T
+with
+path_ids_Lemma (pth : path) : pth.|[ids] = pth.
+Proof.
+  - destruct v; simpl; auto.
+    + by rewrite up_id_internal // tm_ids_Lemma.
+    + rewrite /hsubst /dms_hsubst.
+      f_equal; induction l; simpl; first trivial.
+        by rewrite IHl up_id_internal // dm_ids_Lemma.
+  - destruct t; simpl; auto; by rewrite ?vl_ids_Lemma ?tm_ids_Lemma.
+  - destruct d; simpl.
+    + by rewrite ty_ids_Lemma.
+    + rewrite /hsubst /vls_hsubst.
+      f_equal. induction l; simpl; first trivial.
+        by rewrite IHl vl_ids_Lemma.
+    + by rewrite vl_ids_Lemma.
+  - destruct T; simpl; auto;
+      by rewrite ?ty_ids_Lemma ?up_id_internal // ?ty_ids_Lemma ?path_ids_Lemma.
+  - induction pth; simpl; auto; by rewrite ?vl_ids_Lemma ?path_ids_Lemma.
+Qed.
 
- Lemma vl_rename_comp_Lemma (σ : var → vl) (ξ : var → var) (v : vl) :
-   rename ξ v.[σ] = v.[σ >>> rename ξ]
- with
- tm_rename_comp_Lemma (σ : var → vl) (ξ : var → var) (t : tm) :
-   rename ξ t.|[σ] = t.|[σ >>> rename ξ]
- with
- dm_rename_comp_Lemma (σ : var → vl) (ξ : var → var) (d : dm) :
-   rename ξ d.|[σ] = d.|[σ >>> rename ξ]
- with
- ty_rename_comp_Lemma (σ : var → vl) (ξ : var → var) (T : ty) :
+Lemma vl_comp_rename_Lemma (ξ : var → var) (σ : var → vl) (v : vl) :
+  (rename ξ v).[σ] = v.[ξ >>> σ]
+with
+tm_comp_rename_Lemma (ξ : var → var) (σ : var → vl) (t : tm) :
+  (rename ξ t).|[σ] = t.|[ξ >>> σ]
+with
+dm_comp_rename_Lemma (ξ : var → var) (σ : var → vl) (d : dm) :
+  (rename ξ d).|[σ] = d.|[ξ >>> σ]
+with
+ty_comp_rename_Lemma (ξ : var → var) (σ : var → vl) (T : ty) :
+  (rename ξ T).|[σ] = T.|[ξ >>> σ]
+with
+path_comp_rename_Lemma (ξ : var → var) (σ : var → vl) (pth : path) :
+  (rename ξ pth).|[σ] = pth.|[ξ >>> σ].
+Proof.
+  - destruct v; simpl; auto.
+    + by rewrite tm_comp_rename_Lemma up_comp_ren_subst.
+    + rewrite /hsubst /dms_hsubst.
+      f_equal; induction l; simpl; first trivial.
+        by rewrite IHl dm_comp_rename_Lemma up_comp_ren_subst.
+  - destruct t; simpl; auto;
+      by rewrite ?vl_comp_rename_Lemma ?tm_comp_rename_Lemma.
+  - destruct d; simpl.
+    + by rewrite ty_comp_rename_Lemma.
+    + rewrite /hsubst /vls_hsubst.
+      f_equal. induction l; simpl; first trivial.
+        by rewrite IHl vl_comp_rename_Lemma.
+    + by rewrite vl_comp_rename_Lemma.
+  - destruct T; simpl; auto;
+      rewrite ?ty_comp_rename_Lemma ?path_comp_rename_Lemma;
+        by try rewrite up_comp_ren_subst.
+  - induction pth; simpl; auto;
+      by rewrite ?vl_comp_rename_Lemma ?path_comp_rename_Lemma.
+Qed.
+
+Lemma vl_rename_comp_Lemma (σ : var → vl) (ξ : var → var) (v : vl) :
+  rename ξ v.[σ] = v.[σ >>> rename ξ]
+with
+tm_rename_comp_Lemma (σ : var → vl) (ξ : var → var) (t : tm) :
+  rename ξ t.|[σ] = t.|[σ >>> rename ξ]
+with
+dm_rename_comp_Lemma (σ : var → vl) (ξ : var → var) (d : dm) :
+  rename ξ d.|[σ] = d.|[σ >>> rename ξ]
+with
+ty_rename_comp_Lemma (σ : var → vl) (ξ : var → var) (T : ty) :
   rename ξ T.|[σ] = T.|[σ >>> rename ξ]
- with
- pth_rename_comp_Lemma (σ : var → vl) (ξ : var → var) (pth : path) :
-   rename ξ pth.|[σ] = pth.|[σ >>> rename ξ].
- Proof.
-   - destruct v; simpl; auto.
-     + by rewrite tm_rename_comp_Lemma up_comp_subst_ren_internal;
-         auto using vl_rename_Lemma, vl_comp_rename_Lemma.
-     + f_equal; induction l; simpl; first trivial.
-       by rewrite IHl dm_rename_comp_Lemma
-                  up_comp_subst_ren_internal;
-         auto using vl_rename_Lemma, vl_comp_rename_Lemma.
-   - destruct t; simpl; auto;
-       by rewrite ?vl_rename_comp_Lemma ?tm_rename_comp_Lemma.
-   - destruct d; simpl.
-     + by rewrite ty_rename_comp_Lemma.
-     + f_equal. induction l; simpl; first trivial.
-       by rewrite IHl vl_rename_comp_Lemma.
-     + by rewrite vl_rename_comp_Lemma.
-   - destruct T; simpl; auto;
-       rewrite ?ty_rename_comp_Lemma ?pth_rename_comp_Lemma
-               ?up_comp_subst_ren_internal;
-       auto using vl_rename_Lemma, vl_comp_rename_Lemma.
-   - induction pth; simpl; auto;
-       by rewrite ?vl_rename_comp_Lemma ?pth_rename_comp_Lemma.
- Qed.
+with
+path_rename_comp_Lemma (σ : var → vl) (ξ : var → var) (pth : path) :
+  rename ξ pth.|[σ] = pth.|[σ >>> rename ξ].
+Proof.
+  - destruct v; simpl; auto.
+    + by rewrite tm_rename_comp_Lemma up_comp_subst_ren_internal;
+        auto using vl_rename_Lemma, vl_comp_rename_Lemma.
+    + rewrite /hsubst /dms_hsubst /rename /dms_rename.
+      f_equal; induction l; simpl; first trivial.
+        by rewrite IHl dm_rename_comp_Lemma
+                   up_comp_subst_ren_internal;
+          auto using vl_rename_Lemma, vl_comp_rename_Lemma.
+  - destruct t; simpl; auto;
+      by rewrite ?vl_rename_comp_Lemma ?tm_rename_comp_Lemma.
+  - destruct d; simpl.
+    + by rewrite ty_rename_comp_Lemma.
+    + rewrite /hsubst /vls_hsubst /rename /vls_rename.
+      f_equal. induction l; simpl; first trivial.
+        by rewrite IHl vl_rename_comp_Lemma.
+    + by rewrite vl_rename_comp_Lemma.
+  - destruct T; simpl; auto;
+      rewrite ?ty_rename_comp_Lemma ?path_rename_comp_Lemma
+              ?up_comp_subst_ren_internal;
+      auto using vl_rename_Lemma, vl_comp_rename_Lemma.
+  - induction pth; simpl; auto;
+      by rewrite ?vl_rename_comp_Lemma ?path_rename_comp_Lemma.
+Qed.
 
- Lemma vl_comp_Lemma (σ τ : var → vl) (v : vl) : v.[σ].[τ] = v.[σ >> τ]
- with
- tm_comp_Lemma (σ τ : var → vl) (t : tm) : t.|[σ].|[τ] = t.|[σ >> τ]
- with
- dm_comp_Lemma (σ τ : var → vl) (d : dm) : d.|[σ].|[τ] = d.|[σ >> τ]
- with
- ty_comp_Lemma (σ τ : var → vl) (T : ty) : T.|[σ].|[τ] = T.|[σ >> τ]
- with
- pth_comp_Lemma (σ τ : var → vl) (pth : path) : pth.|[σ].|[τ] = pth.|[σ >> τ].
- Proof.
-   - destruct v; simpl; auto.
-     + by rewrite tm_comp_Lemma up_comp_internal;
-         auto using vl_rename_comp_Lemma, vl_comp_rename_Lemma.
-     + f_equal; induction l; simpl; first trivial.
-       by rewrite IHl dm_comp_Lemma up_comp_internal;
-         auto using vl_rename_comp_Lemma, vl_comp_rename_Lemma.
-   - destruct t; simpl; auto;
-       by rewrite ?vl_comp_Lemma ?tm_comp_Lemma.
-   - destruct d; simpl.
-     + by rewrite ty_comp_Lemma.
-     + f_equal. induction l; simpl; first trivial.
-       by rewrite IHl vl_comp_Lemma.
-     + by rewrite vl_comp_Lemma.
-   - destruct T; simpl; auto;
-       rewrite ?ty_comp_Lemma ?pth_comp_Lemma
-               ?up_comp_internal;
-         auto using vl_rename_comp_Lemma, vl_comp_rename_Lemma.
-   - induction pth; simpl; auto;
-       by rewrite ?vl_comp_Lemma ?pth_comp_Lemma.
- Qed.
+Lemma vl_comp_Lemma (σ τ : var → vl) (v : vl) : v.[σ].[τ] = v.[σ >> τ]
+with
+tm_comp_Lemma (σ τ : var → vl) (t : tm) : t.|[σ].|[τ] = t.|[σ >> τ]
+with
+dm_comp_Lemma (σ τ : var → vl) (d : dm) : d.|[σ].|[τ] = d.|[σ >> τ]
+with
+ty_comp_Lemma (σ τ : var → vl) (T : ty) : T.|[σ].|[τ] = T.|[σ >> τ]
+with
+path_comp_Lemma (σ τ : var → vl) (pth : path) : pth.|[σ].|[τ] = pth.|[σ >> τ].
+Proof.
+  - destruct v; simpl; auto.
+    + by rewrite tm_comp_Lemma up_comp_internal;
+        auto using vl_rename_comp_Lemma, vl_comp_rename_Lemma.
+    + rewrite /hsubst /dms_hsubst.
+      f_equal; induction l; simpl; first trivial.
+        by rewrite IHl dm_comp_Lemma up_comp_internal;
+          auto using vl_rename_comp_Lemma, vl_comp_rename_Lemma.
+  - destruct t; simpl; auto;
+      by rewrite ?vl_comp_Lemma ?tm_comp_Lemma.
+  - destruct d; simpl.
+    + by rewrite ty_comp_Lemma.
+    + rewrite /hsubst /vls_hsubst.
+      f_equal. induction l; simpl; first trivial.
+        by rewrite IHl vl_comp_Lemma.
+    + by rewrite vl_comp_Lemma.
+  - destruct T; simpl; auto;
+      rewrite ?ty_comp_Lemma ?path_comp_Lemma
+              ?up_comp_internal;
+      auto using vl_rename_comp_Lemma, vl_comp_rename_Lemma.
+  - induction pth; simpl; auto;
+      by rewrite ?vl_comp_Lemma ?path_comp_Lemma.
+Qed.
 
- Instance SubstLemmas_vl : SubstLemmas vl.
- Proof.
-   split; auto using vl_rename_Lemma, vl_ids_Lemma, vl_comp_Lemma.
- Qed.
+Instance SubstLemmas_vl : SubstLemmas vl.
+Proof.
+  split; auto using vl_rename_Lemma, vl_ids_Lemma, vl_comp_Lemma.
+Qed.
 
- Instance HSubstLemmas_tm : HSubstLemmas vl tm.
- Proof.
-   split; auto using tm_ids_Lemma, tm_comp_Lemma.
- Qed.
+Instance HSubstLemmas_tm : HSubstLemmas vl tm.
+Proof.
+  split; auto using tm_ids_Lemma, tm_comp_Lemma.
+Qed.
 
- Instance HSubstLemmas_ty : HSubstLemmas vl ty.
- Proof.
-   split; auto using ty_ids_Lemma, ty_comp_Lemma.
- Qed.
+Instance HSubstLemmas_ty : HSubstLemmas vl ty.
+Proof.
+  split; auto using ty_ids_Lemma, ty_comp_Lemma.
+Qed.
 
- Instance HSubstLemmas_dm : HSubstLemmas vl dm.
- Proof.
-   split; auto using dm_ids_Lemma, dm_comp_Lemma.
- Qed.
+Instance HSubstLemmas_dm : HSubstLemmas vl dm.
+Proof.
+  split; auto using dm_ids_Lemma, dm_comp_Lemma.
+Qed.
 
- Instance HSubstLemmas_pth : HSubstLemmas vl path.
- Proof.
-   split; auto using pth_ids_Lemma, pth_comp_Lemma.
- Qed.
+Instance HSubstLemmas_pth : HSubstLemmas vl path.
+Proof.
+  split; auto using path_ids_Lemma, path_comp_Lemma.
+Qed.
+
+Instance HSubstLemmas_vls : HSubstLemmas vl vls.
+Proof.
+  split; trivial.
+  - intros vs. rewrite /hsubst /HSubst_vls /vls_hsubst.
+    induction vs; simpl; first trivial.
+    by rewrite IHvs vl_ids_Lemma.
+  - intros θ η vs. rewrite /hsubst /HSubst_vls /vls_hsubst.
+    induction vs; simpl; first trivial.
+    by rewrite IHvs vl_comp_Lemma.
+Qed.
+
+Instance HSubstLemmas_dms : HSubstLemmas vl dms.
+Proof.
+  split; trivial.
+  - intros ds. rewrite /hsubst /HSubst_dms /dms_hsubst.
+    induction ds; simpl; first trivial.
+    by rewrite IHds dm_ids_Lemma.
+  - intros θ η ds. rewrite /hsubst /HSubst_dms /dms_hsubst.
+    induction ds; simpl; first trivial.
+    by rewrite IHds dm_comp_Lemma.
+Qed.
