theories/synFuncs.v
@@ -5,77 +5,72 @@ This file should not load Iris code to reduce compile times.
 Require Import Dot.tactics.
 Require Export Dot.dotsyn.
 Require Import stdpp.list.
+From iris.base_logic.lib Require Import invariants.
 
-Module SynFuncs (gnameMod: type).
-Import gnameMod.
-Module SynG := Syn gnameMod.
-Export SynG.
+Implicit Types (L T U: ty) (v: vl) (e: tm) (d: dm) (Γ : list ty).
 
-Implicit Types (L T U: ty) (v: vl) (e: tm) (d: dm) (ds: dms) (Γ : list ty).
+(* Fixpoint dms_to_list (ds: dms) : list dm := *)
+(*   match ds with *)
+(*   | dnil => [] *)
+(*   | dcons d ds => d :: dms_to_list ds *)
+(*   end. *)
 
-Fixpoint dms_to_list (ds: dms) : list dm :=
-  match ds with
-  | dnil => []
-  | dcons d ds => d :: dms_to_list ds
-  end.
+(* Fixpoint vls_to_list (vs: vls) : list vl := *)
+(*   match vs with *)
+(*   | vlnil => [] *)
+(*   | vlcons v vs => v :: vls_to_list vs *)
+(*   end. *)
 
-Fixpoint vls_to_list (vs: vls) : list vl :=
-  match vs with
-  | vlnil => []
-  | vlcons v vs => v :: vls_to_list vs
-  end.
+(* (** Reverse lookup. *) *)
+(* Fixpoint indexr {X} (i: nat) (xs: list X) : option X := *)
+(*   match xs with *)
+(*   | [] => None *)
+(*   | x :: xs => *)
+(*     if decide (i = length xs) then Some x else indexr i xs *)
+(*   end. *)
 
-(** Reverse lookup. *)
-Fixpoint indexr {X} (i: nat) (xs: list X) : option X :=
-  match xs with
-  | [] => None
-  | x :: xs =>
-    if decide (i = length xs) then Some x else indexr i xs
-  end.
+(* Definition index_dms (i: label) (ds: dms): option dm := *)
+(*   indexr i (dms_to_list ds). *)
 
-Definition index_dms (i: label) (ds: dms): option dm :=
-  indexr i (dms_to_list ds).
+(* Definition dms_length ds := length (dms_to_list ds). *)
 
-Definition dms_length ds := length (dms_to_list ds).
+(* (** Single-variable substitution, based on the Autosubst1 notation. Priorities copied from s .[ sigma ]. *) *)
+(* Notation "s .[ v /]" := (s .[ v .: var_vl ]) *)
+(*   (at level 2, v at level 200, left associativity, *)
+(*    format "s .[ v /]" ) : subst_scope. *)
 
-(** Single-variable substitution, based on the Autosubst1 notation. Priorities copied from s .[ sigma ]. *)
-Notation "s .[ v /]" := (s .[ v .: var_vl ])
-  (at level 2, v at level 200, left associativity,
-   format "s .[ v /]" ) : subst_scope.
-
-(** Substitute object inside itself (to give semantics to the "self"
-    variable). To use when descending under the [vobj] binder. *)
-Definition selfSubst (ds: dms): dms := ds.[vobj ds/].
+(* (** Substitute object inside itself (to give semantics to the "self" *)
+(*     variable). To use when descending under the [vobj] binder. *) *)
+Definition selfSubst (ds: dms): dms := ds.|[vobj ds/].
 
 Definition objLookup v l d: Prop :=
-  ∃ ds, v = vobj ds ∧ index_dms l (selfSubst ds) = Some d.
+  ∃ ds, v = vobj ds ∧ reverse (selfSubst ds) !! l = Some d.
 Notation "v @ l ↘ d" := (objLookup v l d) (at level 20).
 
-(** Instead of letting obj_opens_to autounfold, provide tactics to show it's deterministic and so on. *)
+(** Instead of letting obj_opens_to autounfold,
+    provide tactics to show it's deterministic and so on. *)
 
 (** Convert environment to substitution. *)
 Definition to_subst (ρ: list vl) i: vl :=
   match ρ !! i with
   | Some v => v
-  | None => var_vl i
+  | None => var_vl (i - length ρ)
   end.
 
-Definition subst_sigma (σ: vls) (ρ: list vl) := vls_to_list (σ.[to_subst ρ]).
+Definition subst_sigma (σ: vls) (ρ: list vl) := σ.|[to_subst ρ].
 
-Definition push_var (σ: vls): vls := vlcons (var_vl 0) σ.[(+1) >>> var_vl].
+Definition push_var (σ: vls) : vls := (var_vl 0) :: σ.|[ren (+1)].
 
-(** Create an identity environment vls.
- * The definition gives the right results but is not ideal to reason about. It
-   is hard to prove it does what it should, and it's likely theorems using it
-   should be rephrased in terms of the translation.
- *)
-Fixpoint idsσ (ρ: list vl): vls :=
-  match ρ with
-  | [] => vlnil
-  | _ :: ρ1 => push_var (idsσ ρ1)
-  end.
+(* (** Create an identity environment vls. *)
+(*  * The definition gives the right results but is not ideal to reason about. It *)
+(*    is hard to prove it does what it should, and it's likely theorems using it *)
+(*    should be rephrased in terms of the translation. *)
+(*  *) *)
+(* Fixpoint idsσ (ρ: list vl): vls := *)
+(*   match ρ with *)
+(*   | [] => vlnil *)
+(*   | _ :: ρ1 => push_var (idsσ ρ1) *)
+(*   end. *)
 
-Definition wkT := toSubst_ty (+1).
-Definition wkV := toSubst_vl (+1).
-
-End SynFuncs.
+(* Definition wkT := toSubst_ty (+1). *)
+(* Definition wkV := toSubst_vl (+1). *)
